Fixed examples

Source/DafnyStandardLibraries/examples/FramesExamples.dfy
@@ -1,5 +1,137 @@
 module FramesExamples {
 
-  
+  import opened Std.Frames
+
+  // A non-trivial example of a recursive data strucutre
+  // using the Validatable trait.
+  // In particular, expressing the Node class invariant
+  // necessary in order to prove termination of recursive methods
+  // is much simpler using ValidComponent().
+
+  @AssumeCrossModuleTermination
+  trait Tree<T> extends Validatable {
+
+    ghost var nodeCount: nat
+
+    method Elements() returns (result: seq<T>)
+      requires Valid()
+      decreases Repr
+      ensures Valid()
+  }
+
+  class Leaf<T> extends Tree<T> {
+
+    constructor () 
+      ensures Valid()
+    {
+      Repr := {this};
+      nodeCount := 0;
+    }
+
+    ghost predicate Valid()
+      reads this, Repr
+      ensures Valid() ==> this in Repr
+      decreases Repr, 0
+    {
+      && this in Repr
+    }
+
+    method Elements() returns (result: seq<T>)
+      requires Valid()
+      decreases Repr
+      ensures Valid()
+    {
+      return [];
+    }
+  }
+
+  class Node<T> extends Tree<T> {
+
+    var value: T
+    var left: Tree<T>
+    var right: Tree<T>
+
+    constructor (left: Tree<T>, value: T, right: Tree<T>) 
+      requires left.Valid()
+      requires right.Valid()
+      requires left.Repr !! right.Repr
+      ensures Valid()
+      ensures this.left == left
+      ensures this.value == value
+      ensures this.right == right
+      ensures fresh(Repr - left.Repr - right.Repr)
+    {
+      this.left := left;
+      this.value := value;
+      this.right := right;
+
+      Repr := {this} + left.Repr + right.Repr;
+      nodeCount := left.nodeCount + right.nodeCount + 1;
+    }
+
+    ghost predicate Valid()
+      reads this, Repr
+      ensures Valid() ==> this in Repr
+      decreases Repr, 0
+    {
+      && this in Repr
+      && ValidComponent(left)
+      && ValidComponent(right)
+      && left.Repr !! right.Repr
+      && nodeCount == left.nodeCount + right.nodeCount + 1
+    }
+
+    method Elements() returns (result: seq<T>)
+      requires Valid()
+      decreases Repr
+      ensures Valid()
+    {
+      result := [value];
+      var leftElements := left.Elements();
+      result := result + leftElements;
+      var rightElements := right.Elements();
+      result := result + rightElements;
+    }
+
+    // Note that Repr CANNOT used as the decreases clause for this method
+    // since it allocates new nodes and hence Repr sets grow,
+    // even if they contain fresh objects.
+    // Instead, it is necessary to define a more domain-specific
+    // termination measure based on what work is being done
+    // (in this case a count of the number of nodes in subtrees)
+    @IsolateAssertions
+    method RotateRight() 
+      requires Valid()
+      modifies Repr
+      decreases nodeCount
+      ensures ValidAndDisjoint()
+    {
+      if left is Node<T> {
+        var leftAsNode := left as Node<T>;
+        
+        var leftValue := leftAsNode.value;
+        var oldRight := right;
+        right := new Node(leftAsNode.right, value, oldRight);
+        left := leftAsNode.left;
+        value := leftAsNode.value;
+
+        // This kind of "bookkeeping" of ghost state
+        // is often necessary.
+        // Repeating it at various points in the control flow
+        // can look duplicative and noisy,
+        // but since it is all ghost state there is no runtime cost,
+        // and it often makes verification cheaper and hence less brittle.
+        Repr := {this} + left.Repr + right.Repr;
+        nodeCount := left.nodeCount + right.nodeCount + 1;
+      }
+
+      if (right is Node<T>) {
+        (right as Node<T>).RotateRight();
+
+        Repr := {this} + left.Repr + right.Repr;
+        nodeCount := left.nodeCount + right.nodeCount + 1;
+      }
+    }
+  }
 
 }
